---
title: "ChatGPT"
source: "https://chatgpt.com/?temporary-chat=true"
author:
  - "[[ChatGPT]]"
published:
created: 2025-09-14
description: "ChatGPT helps you get answers, find inspiration and be more productive. It is free to use and easy to try. Just ask and ChatGPT can help with writing, learning, brainstorming and more."
tags:
  - "clippings"
---
Temporary Chat

`(∘(in)(᛫) = ¬(᛫))` parses as a transformation rule:

- Operator `∘(in)` acts as inversion-context application.
- Operand `(᛫)` is a placeholder or undifferentiated token.
- Result `¬(᛫)` signals negation of that placeholder.

So: **“Applying the `in` -composition operator to any undifferentiated element yields its logical negation.”**

This encodes a meta-rule:

$$
∘_{in}(x) := ¬x
$$

Want me to expand this into a general algebra (closure, associativity, involution properties)?

Define algebra $\mathcal{A} = (\mathcal{U}, \circ_{in}, \neg)$ .

---

**1\. Universe (closure)**

- $\mathcal{U}$ = set of primitive tokens (e.g. $\{\;᛫, a, b, \dots\}$ ).
- Rule:
	$$
	\circ_{in}(x) = \neg x, \quad \forall x \in \mathcal{U}
	$$
- Closure: if $x \in \mathcal{U}$ , then $\neg x \in \mathcal{U}$ .

---

**2\. Associativity**

- For composition:
	$$
	\circ_{in}(\circ_{in}(x)) = \circ_{in}(\neg x) = \neg(\neg x) = x
	$$
- So $\circ_{in}$ is **self-inverse**.
- General associativity check:  
	$(\circ_{in} \circ \circ_{in})(x) = id(x)$ .  
	Thus:
	$$
	\circ_{in} \circ \circ_{in} = id
	$$
- Associativity holds trivially for repeated application since it reduces to identity or $\circ_{in}$ .

---

**3\. Involution**

- Involution property:
	$$
	\neg(\neg x) = x
	$$
- Therefore $\circ_{in}$ is an involution operator.

---

**4\. Algebraic structure**

- $\mathcal{A}$ is a **Boolean-like involutive algebra** with a single unary operator.
- It forms a group of order 2 under function composition:  
	$\{ id, \circ_{in} \}$ .

---

**5\. Generalized laws**

- Identity: $\circ_{in}^0(x) = x$ .
- Negation: $\circ_{in}^1(x) = \neg x$ .
- Periodicity: $\circ_{in}^{2n}(x) = x$ , $\circ_{in}^{2n+1}(x) = \neg x$ .

---

Do you want me to extend this beyond unary into a **full algebra with binary operations** (like meet/join → full Boolean algebra), or keep it minimal as a unary involutive system?

Minimal unary involutive system:

---

**System $\mathcal{I}$**

- Universe: $\mathcal{U}$ .
- Operator: $\circ_{in} : \mathcal{U} \to \mathcal{U}$ .
- Rule: $\circ_{in}(x) = \neg x$ .

---

**Axioms**

1. **Closure:** $\forall x \in \mathcal{U}, \neg x \in \mathcal{U}$ .
2. **Involution:** $\neg(\neg x) = x$ .
3. **Identity pairing:** Each element $x$ is uniquely paired with $\neg x$ .
4. **No fixed points (unless degenerate):** $x = \neg x \implies x$ is a special self-dual element.

---

**Structure**

- The operator set $\{id, \circ_{in}\}$ forms a group of order 2 under composition.
- Each orbit of $\circ_{in}$ has size 2: $\{x, \neg x\}$ .
- If a self-dual element exists, its orbit has size 1.

---

**Consequences**

- Periodicity: $\circ_{in}^{2n}(x) = x$ , $\circ_{in}^{2n+1}(x) = \neg x$ .
- Associativity is trivial because only one unary operator exists.

---

This is the **simplest nontrivial algebraic system**: a set partitioned into disjoint 2-cycles (plus optional 1-cycles for self-duals).

Do you want me to classify this system formally as a **Z₂-action on a set**?

Then we extend the unary involution into a **Heyting algebra with involution** (a.k.a. *De Morgan–Heyting algebra*).

---

### 1\. Base Heyting structure

A Heyting algebra $(H, \wedge, \vee, \to, 0, 1)$ :

- $(H, \wedge, \vee, 0, 1)$ is a bounded distributive lattice.
- Implication $\to$ satisfies:
	$$
	a \wedge b \leq c \quad \text{iff} \quad a \leq (b \to c).
	$$
- Pseudocomplement (intuitionistic negation):
	$$
	\neg a := (a \to 0).
	$$

---

### 2\. Involution operator from your seed

We introduce an **involutive negation** operator $\circ_{in}$ , extending your rule:

$$
\circ_{in}(a) = \neg a
$$

with the **axiom**

$$
\circ_{in}(\circ_{in}(a)) = a.
$$

This is stronger than ordinary Heyting negation, where only $\neg\neg a \geq a$ holds.

---

### 3\. Resulting algebra

The structure becomes:

$$
(H, \wedge, \vee, \to, 0, 1, \circ_{in})
$$

with properties:

1. **Closure:** $\circ_{in}(a) \in H$ .
2. **Involution:** $\circ_{in}(\circ_{in}(a)) = a$ .
3. **De Morgan laws (provable here):**
	- $\circ_{in}(a \vee b) = \circ_{in}(a) \wedge \circ_{in}(b)$
	- $\circ_{in}(a \wedge b) = \circ_{in}(a) \vee \circ_{in}(b)$
4. **Residuality:** $a \wedge b \leq c \iff a \leq (b \to c)$ .

---

### 4\. Difference from Boolean algebra

- Boolean: $a \vee \neg a = 1$ (law of excluded middle).
- Heyting with involution: not necessarily true.
	- Only guarantees $a \vee \neg a \leq 1$ .
	- Thus supports **constructive logic with strong negation** (Nelson logic).

---

### 5\. Interpretive frame

- Ordinary Heyting algebra: models intuitionistic logic.
- Adding involution: yields **Nelson algebras**, semantics for constructive logic with strong negation.
- Your seed operator $(\circ_{in}(᛫) = ¬᛫)$ thus scales to a **Nelson–Heyting system**.

---

Do you want me to **write out the sequent calculus / natural deduction rules** corresponding to this algebra (so you see the logic-level effect of introducing $\circ_{in}$ )?

Here is the logic layer corresponding to a **Heyting algebra with involutive negation** (a Nelson–Heyting system).

---

## 1\. Core intuitionistic rules (Heyting base)

Sequents are of the form $\Gamma \vdash A$ .

- **Identity / Cut:**
	$$
	A \vdash A, 
	\quad
	\frac{\Gamma \vdash A \quad \Delta, A \vdash B}{\Gamma, \Delta \vdash B}
	$$
- **Conjunction ( $\wedge$ ):**
	- Intro: $\frac{\Gamma \vdash A \quad \Gamma \vdash B}{\Gamma \vdash A \wedge B}$ .
	- Elim: $\frac{\Gamma \vdash A \wedge B}{\Gamma \vdash A}$ ,  
		$\frac{\Gamma \vdash A \wedge B}{\Gamma \vdash B}$ .
- **Disjunction ( $\vee$ ):**
	- Intro: $\frac{\Gamma \vdash A}{\Gamma \vdash A \vee B}$ ,  
		$\frac{\Gamma \vdash B}{\Gamma \vdash A \vee B}$ .
	- Elim: $\frac{\Gamma \vdash A \vee B \quad \Delta, A \vdash C \quad \Theta, B \vdash C}{\Gamma,\Delta,\Theta \vdash C}$ .
- **Implication ( $\to$ ):**
	- Intro: $\frac{\Gamma, A \vdash B}{\Gamma \vdash A \to B}$ .
	- Elim (modus ponens): $\frac{\Gamma \vdash A \to B \quad \Delta \vdash A}{\Gamma,\Delta \vdash B}$ .
- **Falsum ( $0$ ):**
	- Ex falso: $\frac{\Gamma \vdash 0}{\Gamma \vdash A}$ .

---

## 2\. Intuitionistic negation (pseudo-negation)

Defined as:

$$
\neg A := (A \to 0)
$$

Rules:

- Intro: $\frac{\Gamma, A \vdash 0}{\Gamma \vdash \neg A}$ .
- Elim: $\frac{\Gamma \vdash A \quad \Delta \vdash \neg A}{\Gamma,\Delta \vdash 0}$ .

This only guarantees **double negation weakening**:

$$
A \vdash \neg\neg A
$$

but not the converse.

---

## 3\. Strong involutive negation (∘in\\circ\_{in})

Now add your operator $\circ_{in}$ with involution axioms:

$$
\circ_{in}(\circ_{in}(A)) \equiv A.
$$

### Rules:

- **Intro (symmetry):**  
	$\frac{\Gamma \vdash A}{\Gamma \vdash \circ_{in}(\circ_{in}A)}$ .
- **Involution (collapse):**  
	$\frac{\Gamma \vdash \circ_{in}(\circ_{in}A)}{\Gamma \vdash A}$ .
- **De Morgan laws (admissible):**
	$$
	\circ_{in}(A \wedge B) \vdash \circ_{in}A \vee \circ_{in}B,
	\quad
	\circ_{in}(A \vee B) \vdash \circ_{in}A \wedge \circ_{in}B.
	$$
- **Consistency principle:**  
	$\vdash \neg(A \wedge \circ_{in}A)$ .  
	(prevents collapse to triviality).

---

## 4\. Natural deduction sketch

- From $A$ , assume $\circ_{in}A$ . Derive contradiction, conclude $\neg A$ .
- From $\circ_{in}A$ , derive $\neg A$ .
- From $\neg A$ , not always $\circ_{in}A$ (distinguishes pseudo-negation from involutive one).

So the system has **two negations**:

- $\neg$ = pseudo-negation (intuitionistic).
- $\circ_{in}$ = strong involution (your operator).

---

## 5\. Logic-level characterization

- This yields **Nelson constructive logic with strong negation**.
- Semantics: exactly your “Heyting + involution” algebra.
- Proof-theoretic effect: we gain full symmetry $\circ_{in}\circ_{in}A \leftrightarrow A$ , but not excluded middle.

---

Do you want me to **lay out the full sequent rules side by side for both negations** ( $\neg$ vs $\circ_{in}$ ), so you see exactly how they differ operationally?

Here is a side-by-side sequent system showing the difference between **intuitionistic negation** ( $\neg$ ) and your **involutive negation** ( $\circ_{in}$ ).

---

## 1\. Intuitionistic negation (¬A:=A→0\\neg A:= A \\to 0)

- **Intro (right rule):**
	$$
	\frac{\Gamma, A \vdash 0}{\Gamma \vdash \neg A}
	$$
- **Elim (left rule / contradiction):**
	$$
	\frac{\Gamma \vdash A \quad \Delta \vdash \neg A}{\Gamma,\Delta \vdash 0}
	$$
- **Double negation law (weak):**
	$$
	A \vdash \neg\neg A
	$$
	Converse $\neg\neg A \vdash A$ does not generally hold.

---

## 2\. Strong involutive negation (∘in\\circ\_{in})

- **Intro (reflection):**
	$$
	\frac{\Gamma \vdash A}{\Gamma \vdash \circ_{in}(\circ_{in}A)}
	$$
- **Collapse (involution):**
	$$
	\frac{\Gamma \vdash \circ_{in}(\circ_{in}A)}{\Gamma \vdash A}
	$$
- **Contradiction (De Morgan):**
	$$
	\frac{\Gamma \vdash A \quad \Delta \vdash \circ_{in}A}{\Gamma,\Delta \vdash 0}
	$$
- **De Morgan laws (admissible):**
	$$
	\circ_{in}(A \wedge B) \vdash \circ_{in}A \vee \circ_{in}B
	$$
	 
	$$
	\circ_{in}(A \vee B) \vdash \circ_{in}A \wedge \circ_{in}B
	$$
- **Strong double negation:**
	$$
	A \dashv\vdash \circ_{in}(\circ_{in}A)
	$$

---

## 3\. Key contrasts

| Aspect | $\neg$ (intuitionistic) | $\circ_{in}$ (strong involution) |
| --- | --- | --- |
| Definition | $A \to 0$ | Primitive unary operator |
| Double negation | Only $A \vdash \neg\neg A$ | $A \dashv\vdash \circ_{in}(\circ_{in}A)$ |
| Excluded middle | Not valid | Still not valid |
| Contradiction handling | $\Gamma \vdash A, \Delta \vdash \neg A \implies 0$ | Same with $\circ_{in}$ |
| De Morgan laws | Do not generally hold | Hold as theorems |

---

This shows the operational split:

- $\neg$ = **pseudo-negation** (intuitionistic, weaker, monotone).
- $\circ_{in}$ = **involutive strong negation** (gives De Morgan duality and symmetry).

---

Do you want me to now **embed both into one unified calculus** (a Nelson-style sequent system with two negations side by side), so inference rules explicitly allow *both kinds of negation at once*?

Here is a **unified Nelson-style sequent calculus** where both **intuitionistic negation** ( $\neg$ ) and **involutive negation** ( $\circ_{in}$ ) coexist.

---

## Unified Sequent Calculus NEL¬,∘\\mathsf{NEL}\_{\\neg,\\circ}

Sequents: $\Gamma \vdash A$ .  
Language: $\wedge, \vee, \to, 0, 1, \neg, \circ_{in}$ .

---

## 1\. Structural rules

- **Identity:** $A \vdash A$ .
- **Cut:** $\dfrac{\Gamma \vdash A \quad \Delta, A \vdash B}{\Gamma, \Delta \vdash B}$ .
- Weakening, contraction, exchange as usual.

---

## 2\. Heyting core

- Conjunction, disjunction, implication, and falsum rules as in standard intuitionistic sequent calculus (already written in earlier step).

---

## 3\. Intuitionistic negation rules (¬\\neg)

$$
\neg A := (A \to 0)
$$
- **Intro:** $\dfrac{\Gamma, A \vdash 0}{\Gamma \vdash \neg A}$ .
- **Elim:** $\dfrac{\Gamma \vdash A \quad \Delta \vdash \neg A}{\Gamma, \Delta \vdash 0}$ .
- **Weak double negation:** $A \vdash \neg\neg A$ .

---

## 4\. Strong involutive negation rules (∘in\\circ\_{in})

- **Involution:**
	$$
	\dfrac{\Gamma \vdash A}{\Gamma \vdash \circ_{in}\circ_{in}A}
	\quad\quad
	\dfrac{\Gamma \vdash \circ_{in}\circ_{in}A}{\Gamma \vdash A}
	$$
- **Contradiction:**
	$$
	\dfrac{\Gamma \vdash A \quad \Delta \vdash \circ_{in}A}{\Gamma,\Delta \vdash 0}
	$$
- **De Morgan admissibles:**
	$$
	\circ_{in}(A \wedge B) \vdash \circ_{in}A \vee \circ_{in}B
	$$
	 
	$$
	\circ_{in}(A \vee B) \vdash \circ_{in}A \wedge \circ_{in}B
	$$
- **Strong double negation equivalence:**
	$$
	A \dashv\vdash \circ_{in}\circ_{in}A
	$$

---

## 5\. Interaction principles between ¬\\neg and ∘in\\circ\_{in}

This is what makes it **unified Nelson-style**:

- From strong to weak:
	$$
	\circ_{in}A \vdash \neg A
	$$
	(every strong negation entails pseudo-negation).
- Converse does not generally hold:
	$$
	\neg A \nvdash \circ_{in}A
	$$
- Consistency axiom:
	$$
	\vdash \neg(A \wedge \circ_{in}A)
	$$
	(prevents trivialization).

---

## 6\. Meta-theoretic view

- This calculus is sound and complete w.r.t. **Nelson algebras** (Heyting algebras + involution).
- $\neg$ is constructive/intuitionistic negation.
- $\circ_{in}$ is strong, symmetric negation with full De Morgan duality.
- They cohabit: $\neg$ captures failure-to-prove, $\circ_{in}$ captures explicit contradiction.

---

Would you like me to **draw the full proof net (Gentzen tree) for a key sequent like $\circ_{in}A \vdash \neg A$**, so you can see the mechanics of how strong negation entails intuitionistic negation step by step?

I’m tasked with drawing a Gentzen tree for the sequent ∘in A ⊢ ¬A. The structure must be minimal and step-by-step.

1. Start with the premise ∘in A ⊢ ∘in A (Identity rule).
2. Assume A: ∘in A, A ⊢ 0 (using contradiction for strong negation).
3. Conclude ¬A by negation introduction, discharging assumption of A.

I’ll stick to a clear proof net using natural deduction rules.

I can proceed by using →-introduction. From step 2, I derive ∘in A ⊢ A → 0, which means negation of A. So the sequent becomes ∘in A ⊢ ¬A.

In Gentzen style, I’ll need to show the rules clearly—labeled Id, and contradiction. Since I haven't defined a specific ∘-Left rule, I’ll focus on using →R in the derivation instead.

To derive ∘A ⊢ ¬A, I’ll first use the identity rule to get:

- ∘A, A ⊢ A
- ∘A, A ⊢ ∘A

Next, I’ll apply the contradiction rule to these two results to derive ∘A, A ⊢ 0. Then, using →R, I discharge A and obtain ∘A ⊢ A → 0, which is ¬A.

Here’s the formal Gentzen tree:

We start by annotating rule names: (Id), (Weakening), and (Contr\_∘). We used structural rules like weakening implicitly to have both assumptions present. Identity can be extended with extra assumptions, as seen in this case.

The immediate result is:

1. Assume ∘A \[premise\]
2. Assume A \[assumption\]
3. From 2 and 1, derive 0 by the contradiction rule
4. Discharge 2, and conclude ¬A by ¬-intro.

Thus, ∘A ⊢ ¬A. The formula is minimal but mathematically clear.

Done

Result: $\circ_{in}A \vdash \neg A$ .

Gentzen tree:

$$
\infer[\to\!R]{\circ_{in}A \vdash A \to 0}{
  \infer[\mathrm{Contr}_{\circ}]{\circ_{in}A, A \vdash 0}{
    \infer[\mathrm{Id}]{\circ_{in}A, A \vdash A}{} 
    \quad
    \infer[\mathrm{Id}]{\circ_{in}A, A \vdash \circ_{in}A}{}
  }
}
$$

Rule notes:

- $\mathrm{Id}$ : identity with context.
- $\mathrm{Contr}_{\circ}$ : from $\Gamma \vdash A$ and $\Delta \vdash \circ_{in}A$ infer $\Gamma,\Delta \vdash 0$ .
- $\to R$ : discharge $A$ on the left to conclude $A \to 0$ (i.e., $\neg A$ ).

Natural deduction version:

1. $\circ_{in}A$ premise.
2. Assume $A$ .
3. From 1 and 2 derive $0$ by $\mathrm{Contr}_{\circ}$ .
4. Discharge 2. Conclude $A \to 0$ i.e. $\neg A$ .

Yes. Written stepwise:

1. Start with definition:
	$$
	\circ_{in}(x) = \neg x
	$$
2. Apply again:
	$$
	\circ_{in}(\circ_{in}(x)) = \circ_{in}(\neg x)
	$$
3. Expand:
	$$
	\circ_{in}(\neg x) = \neg(\neg x)
	$$
4. Involutive law:
	$$
	\neg(\neg x) = x
	$$

Thus:

$$
\circ_{in}(\circ_{in}(x)) = x
$$

This makes $\circ_{in}$ a **true involution**: order-2 operator.  
Every element sits in a **2-cycle orbit** $\{x, \circ_{in}(x)\}$ , unless $x$ is self-dual ( $x = \circ_{in}(x)$ ), in which case the orbit collapses to a singleton.

Do you want me to show how this “cycle of analysis” generalizes into a **Z₂-action on the lattice of propositions** (the algebraic symmetry view)?

this is what gemini said, im not sure gemini is correct, what do you think? That's a really interesting way to describe involution! It's a great analogy, but there's a slight misunderstanding in the way you've applied the concept. Let's break down what involution is and then look at the logical operators you've used. ### What is Involution? In mathematics, an \*\*involution\*\* is a function or operation that is its own inverse. This means that if you apply the function twice to any element, you get the original element back. The most common way to write this is: $f(f(x)) = x$ A great example of this is the \*\*reciprocal function\*\* ($f(x) = 1/x$). If you take the reciprocal of a number, say 5, you get $1/5$. If you then take the reciprocal of $1/5$, you get 5 again, which is the original number. So, $f(f(5)) = 5$. --- ### The Logical Operator of Negation The logical operator you used, \*\*negation\*\* ($¬$), is a perfect example of an involution. Negation simply flips the truth value of a statement. \* If a statement is true, its negation is false. \* If a statement is false, its negation is true. Applying negation twice brings you back to the original truth value. This is known as the \*\*Law of Double Negation\*\*. $¬(¬x) = x$ For example, if you say "The sky is blue" (which is true), its negation is "The sky is not blue" (false). The negation of that is "It is not the case that the sky is not blue," which is just a convoluted way of saying "The sky is blue" (true). --- ### Your Equation You've combined these concepts in an interesting way, but the equation `∘ᵢₙ(¬x) = ¬(¬x) = x` isn't quite right. The notation `∘ᵢₙ(x)` seems to represent an involution, but you're trying to apply it to `¬x`. The correct way to represent the concept is that the function itself, `∘ᵢₙ`, is an involution. So, `∘ᵢₙ(∘ᵢₙ(x))` is correct because it shows the involution applied to a variable twice. The result is `x`. However, the part `∘ᵢₙ(¬x) = ¬(¬x)` is where the logic gets mixed up. It's like you're stating that the involution of a negated value is the same as a double negation. While both operations are involutions and produce the same result, the first part of the equation isn't how we'd typically write it mathematically. So, the core of your statement, that \*\*applying an involution twice brings you back to the start\*\*, is absolutely correct. Your analogy of it being a "cycle of analysis" is a very insightful way to think about it, especially in fields like logic or signal processing where a process is reversed and then reversed again to recover the original state.

Gemini is mixing two different things. Let’s separate them cleanly.

---

### 1\. Involution (general definition)

A map $f$ is involutive if

$$
f(f(x)) = x
$$

for all $x$ . Nothing more, nothing less.

---

### 2\. Negation in classical logic

Negation is a standard example of involution:

$$
\neg(\neg x) = x.
$$

---

### 3\. Your operator ∘in\\circ\_{in}

You defined:

$$
\circ_{in}(x) = \neg x.
$$

Therefore:

$$
\circ_{in}(\circ_{in}(x)) = \circ_{in}(\neg x) = \neg(\neg x) = x.
$$

This is entirely correct. You are not “mixing” involution with negation—you are explicitly **identifying** $\circ_{in}$ with negation.

---

### 4\. Gemini’s critique

Gemini says:

- It’s right that $\circ_{in}$ is an involution.
- But wrong to write $\circ_{in}(\neg x) = \neg(\neg x)$ .

That’s a mistake on Gemini’s side. Because under your definition $\circ_{in}(x) = \neg x$ , substitution gives:

$$
\circ_{in}(\neg x) = \neg(\neg x).
$$

That is a legitimate direct calculation.

---

### 5\. The real subtlety

- In **classical logic**, $\neg\neg x = x$ , so $\circ_{in}$ is trivially involutive.
- In **intuitionistic logic**, only $x \vdash \neg\neg x$ holds; the equivalence $\neg\neg x \equiv x$ does not.
- That’s why, in constructive settings, we distinguish between pseudo-negation $\neg$ and a strong involutive negation like $\circ_{in}$ .

---

### Verdict

Your formulation is correct **if $\circ_{in}$ is defined as classical negation**.  
Gemini’s correction misreads your step $\circ_{in}(\neg x) = \neg(\neg x)$ . That step follows directly from your definition, so there is no error.

---

Do you want me to show explicitly **how this breaks in a Heyting algebra** (why $\neg\neg x = x$ fails there unless you enforce involution separately)?

Yes. The breakdown is structural.

---

## 1\. Reminder: Heyting negation

In a Heyting algebra $H$ ,

$$
\neg x := (x \to 0)
$$

where $0$ is bottom.

So:

- $x \wedge \neg x = 0$ .
- But $x \vee \neg x = 1$ is **not guaranteed** (excluded middle fails).

---

## 2\. Double negation in Heyting

Compute:

$$
\neg\neg x = ( (x \to 0) \to 0 ).
$$

We always have:

$$
x \leq \neg\neg x.
$$

This is because if $x$ holds, then assuming $\neg x$ would force $0$ , so $x$ entails $\neg\neg x$ .

But the converse $\neg\neg x \leq x$ does **not hold in general**.

---

## 3\. Concrete counterexample: open sets

Let the Heyting algebra be the lattice of open subsets of a topological space, with:

- meet = intersection,
- join = union,
- implication $U \to V$ = interior( $U^c \cup V$ ).  
	Negation:
$$
\neg U = \text{interior}(U^c).
$$

Take $X = \mathbb{R}$ with standard topology.  
Let $U = (0,1)$ .

- Compute $\neg U = \text{int}(\mathbb{R} \setminus (0,1)) = (-\infty,0] \cup [1,\infty)$ (open interior gives $(-\infty,0)\cup(1,\infty)$ ).
- Then $\neg\neg U = \text{int}(\mathbb{R} \setminus ((-\infty,0)\cup(1,\infty))) = \text{int}([0,1]) = (0,1)$ .

Here we actually recover $U$ .

But if we choose $U = \{0\}$ (not open), then $\neg U = \mathbb{R}\setminus\{0\}$ , interior is still $\mathbb{R}\setminus\{0\}$ , and

$$
\neg\neg U = \text{int}(\mathbb{R}\setminus (\mathbb{R}\setminus\{0\})) = \text{int}(\{0\}) = \emptyset.
$$

So $\neg\neg U = \emptyset \neq U$ .

---

## 4\. General pattern

- Always: $x \leq \neg\neg x$ .
- Sometimes: strict inequality, $\neg\neg x > x$ .
- That is the constructive gap.

---

## 5\. Enforcing involution

If we postulate $\circ_{in}(x) := \neg x$ **and add the axiom**

$$
\circ_{in}\circ_{in}(x) = x,
$$

then we collapse every Heyting algebra into a Boolean algebra (since double negation becomes equality, restoring excluded middle).

Alternative: allow $\circ_{in}$ as a **separate operator** distinct from $\neg$ . That yields a **Nelson algebra** (Heyting + involution).

---

So: **the failure of $\neg\neg x = x$ in Heyting** is precisely why intuitionistic negation cannot serve as your $\circ_{in}$ unless you collapse into Boolean logic.

---

Do you want me to **map this directly into sequent calculus rules** showing why $\neg\neg A \vdash A$ is not derivable intuitionistically?

Alright. Let’s pin this down syntactically in the **intuitionistic sequent calculus (LJ)**.

---

## 1\. Negation as abbreviation

In LJ, negation is defined:

$$
\neg A := A \to \bot
$$

So the sequent

$$
\neg\neg A \vdash A
$$

expands to

$$
((A \to \bot) \to \bot) \vdash A.
$$

---

## 2\. Attempted derivation

We want a derivation of $A$ on the right, given assumption $(A \to \bot) \to \bot$ on the left.

- To derive $A$ on the right in LJ, we either need $A$ on the left already (identity axiom), or a construction via $\to L$ or $\to R$ .
- But our only assumption is $(A \to \bot) \to \bot$ .

---

## 3\. Applying implication-left (→L\\to L)

Rule:

$$
\frac{\Gamma \vdash B \quad \Delta, C \vdash D}{\Gamma,\Delta, (B \to C) \vdash D}
$$

Take $B = A \to \bot, \; C = \bot$ . Then the assumption $(A \to \bot) \to \bot$ fits.

So to use it we need subproofs:

1. $\Gamma \vdash A \to \bot$ .
2. $\Delta, \bot \vdash A$ .
- Subproof 2: From $\bot$ we can derive anything, so that’s fine.
- Subproof 1: To derive $A \to \bot$ , we’d need to assume $A$ and derive $\bot$ .

But no assumption of $A$ is available—we only have $(A \to \bot) \to \bot$ . We cannot reach $\bot$ intuitionistically from just that.

So the derivation stalls.

---

## 4\. Classical fix

If we had **classical rule** (double-negation elimination or reductio), we could close the gap:

$$
\frac{\Gamma, \neg A \vdash \bot}{\Gamma \vdash A}
$$

This allows you to conclude $A$ from $\neg\neg A$ .  
But this rule is absent in LJ.

---

## 5\. Conclusion

Thus:

- In **LJ** (intuitionistic sequent calculus), $\neg\neg A \vdash A$ is **not derivable**.
- In **LK** (classical sequent calculus), the additional classical rules make it derivable.

This mirrors the algebraic fact: Heyting algebras validate only $A \vdash \neg\neg A$ , not the converse.

---

Do you want me to **explicitly show the LK proof tree for $\neg\neg A \vdash A$**, so you can see how the classical step (excluded middle / reductio) closes what LJ cannot?

Yes. Let’s write out the **LK derivation** (classical sequent calculus, Gentzen style) of

$$
\neg\neg A \;\vdash\; A
$$

---

## 1\. Expand negation

$\neg A := A \to \bot$ .  
So $\neg\neg A = (A \to \bot) \to \bot$ .  
Sequent becomes:

$$
((A \to \bot) \to \bot) \;\vdash\; A.
$$

---

## 2\. Classical rule needed

In **LK**, we have *reductio ad absurdum* encoded in the rule:

$$
\frac{\Gamma, \neg A \vdash \bot}{\Gamma \vdash A}
\quad (\text{¬¬-elim / classical})
$$

This is not available in LJ.

---

## 3\. Proof tree (LK)

1. **Assume** $\neg\neg A$ on the left.  
	Goal: derive $A$ .
2. Use *reductio*:
	- Temporarily assume $\neg A$ .
	- With $\neg\neg A$ and $\neg A$ , derive $\bot$ .
	- Discharge assumption, conclude $A$ .

---

### Explicit tree

- In the $\to L$ step, we apply the assumption $\neg\neg A = (A \to \bot) \to \bot$ to the temporary assumption $\neg A = A \to \bot$ , yielding $\bot$ .
- Then by the classical negation elimination rule, from $\neg\neg A$ and the reductio step we conclude $A$ .

---

## 4\. Why this closes the gap

- LJ lacks the $\neg$ -elimination step. It only has $\neg A := A \to 0$ , no way to discharge a temporary assumption of $\neg A$ to conclude $A$ .
- LK explicitly allows this. That is exactly where double-negation elimination enters.

---

Do you want me to **draw the corresponding LK proof net (tree with cut-elimination style)** so the *classical step* is visually distinct from the purely structural intuitionistic steps?

Here is the **LK proof net (tree)** for

$$
\neg\neg A \;\vdash\; A
$$

with the **classical step marked**.

---

### 1\. Negation expansion

$\neg A := A \to \bot$ .  
$\neg\neg A = (A \to \bot) \to \bot$ .

So the sequent is:

$$
((A \to \bot) \to \bot) \;\vdash\; A.
$$

---

### 2\. LK proof tree

---

### 3\. Explanation of nodes

- **(→L):** Application of implication-left to the assumption $(A \to \bot) \to \bot$ .  
	It takes as input:
	- Proof of $(A \to \bot)$ .
	- Proof of $\bot$ from that.
- **Id:** Identity axiom for $A \to \bot$ .
- **ex falso:** From $\bot$ , derive $\bot$ (trivial, but shows bottom is absorbing).
- **¬¬E (classical step):** From the contradiction that arises under assumption $\neg A$ , discharge and conclude $A$ . This is the **non-intuitionistic rule**.

---

### 4\. Key contrast

- Up to the (→L) node, the structure is **intuitionistic**.
- The **discharge of $\neg A$** to conclude $A$ is the **classical-only move**.  
	That is why LJ stalls at $\neg\neg A \vdash A$ , while LK succeeds.

---

Do you want me to generalize this into a **visual schema** showing *where* intuitionistic LK rules stop versus where the extra classical rule plugs in (so you can see the “fault line”)?